dataplane/Examples/Traces_op.thy
@@ -3,6 +3,7 @@ theory Traces_op
 imports
   Dataplane.Timely_Infrastructure
   Source_op
+  Set_op
 begin
 
 corec traces_op where
@@ -12,8 +13,6 @@ corec traces_op where
    (Set.filter (\<lambda> f. f p \<noteq> LNil) S)) in 
    Choice (cimage (\<lambda> x. Write (traces_op ((\<lambda> f. f(p := ltl (f p))) ` {f \<in> S. lhd (f p) = x})) p x) hds))
    c\<UU>))"
-
-term "traces_op { f.  (\<forall> p. ldistinct (f p) \<and> lset (f p) \<subseteq> S) }"
 
 lemma step_traces_op_elim:
   assumes "step io (traces_op S) op"
@@ -192,6 +191,14 @@ lemma
       done
     done
   done
+
+thm set_spec_op_trace_eq_set_spec_op_trace_alt
+thm set_op_bisim_set_spec_op
+
+
+lemma
+  "wtraced (traces_op { f.  (\<forall> p. ldistinct (f p) \<and> lset (f p) \<subseteq> S - S') }) ios \<Longrightarrow>
+   "
 
 
 end
